MLS.Parser.fsti
@@ -4,16 +4,15 @@ open MLS.Bytes
 
 (*** Basic definitions ***)
 
-let rec is_suffix_explicit (suffix:bytes) (buf:bytes) (prefixes:list bytes): Tot Type0 (decreases prefixes) =
-  match prefixes with
-  | [] -> suffix == buf
-  | h::t -> is_suffix_explicit (bytes_concat h suffix) buf t
-let is_suffix (suffix:bytes) (buf:bytes) = exists prefixes. is_suffix_explicit suffix buf prefixes
+val add_prefixes: #bytes:Type0 -> {|bytes_like bytes|} -> list bytes -> bytes -> bytes
+let is_suffix (#bytes:Type0) {|bytes_like bytes|} (suffix:bytes) (buf:bytes) = exists prefixes. buf == add_prefixes prefixes suffix
 
-type suffix_of (b:bytes) = suf:bytes{is_suffix suf b}
-type extension_of (suf:bytes) = b:bytes{is_suffix suf b}
-type bare_parser (a:Type) = b:bytes -> option (a & suffix_of b)
-type bare_serializer (a:Type) = x:a -> suffix:bytes -> extension_of suffix
+type suffix_of (#bytes:Type0) {|bytes_like bytes|} (b:bytes) = suf:bytes{is_suffix suf b}
+type extension_of (#bytes:Type0) {|bytes_like bytes|} (suf:bytes) = b:bytes{is_suffix suf b}
+
+type bare_parser (bytes:Type0) {|bytes_like bytes|} (a:Type) = b:bytes -> option (a & suffix_of b)
+//type bare_serializer (bytes:Type0) {|bytes_like bytes|} (a:Type) = x:a -> suffix:bytes -> extension_of suffix
+type bare_serializer (bytes:Type0) {|bytes_like bytes|} (a:Type) = x:a -> list bytes
 
 /// What is the reason behind `parser_serializer_unit` and `parser_serializer`?
 /// In some functions (such as `pse_list` which is used to build `ps_seq` or `ps_bytes`),
@@ -33,62 +32,47 @@ type bare_serializer (a:Type) = x:a -> suffix:bytes -> extension_of suffix
 /// They are named `parser_serializer_unit` / `parser_serializer` and not `parser_serializer` / `parser_serializer_nonempty`
 /// because `parser_serializer_nonempty` is ugly, and it's the type that is the most used by the user.
 
-noeq type parser_serializer_unit (a:Type) = {
-  parse: bare_parser a;
-  serialize: bare_serializer a;
+noeq type parser_serializer_unit (bytes:Type0) {|bytes_like bytes|} (a:Type) = {
+  parse: bare_parser bytes a;
+  serialize: bare_serializer bytes a;
   parse_serialize_inv: x:a -> suffix:bytes -> Lemma (
-    parse (serialize x suffix) == Some (x, suffix)
+    parse (add_prefixes (serialize x) suffix) == Some (x, suffix)
   );
   serialize_parse_inv: buf:bytes -> Lemma (
     match parse buf with
-    | Some (x, suffix) -> buf == serialize x suffix
+    | Some (x, suffix) -> buf == add_prefixes (serialize x) suffix
     | None -> True
   );
-  parse_no_lookahead: b1:bytes -> b2:bytes -> Lemma (
-    True
-    //bytes_concat_length b1 b2;
-    //match parse b1 with
-    //| Some (x, l) -> parse (bytes_concat b1 b2) == Some (x, l)
-    //| None -> True
-  )
-  //parse_no_lookahead: b1:bytes -> b2:bytes -> Lemma
-  //  (requires (
-  //    match parse b1 with
-  //    | Some (_, l) -> l <= bytes_length b2 /\ (bytes_slice b1 0 l == bytes_slice b2 0 l)
-  //    | None -> True
-  //  ))
-  //  (ensures (
-  //    match parse b1 with
-  //    | Some (x1, l1) -> begin
-  //      match parse b2 with
-  //      | Some (x2, l2) -> x1 == x2 /\ l1 == l2
-  //      | None -> False
-  //    end
-  //    | None -> True
-  //  ))
 }
 
-let is_not_unit (#a:Type) (ps_a:parser_serializer_unit a) = ps_a.parse bytes_empty == None
-let parser_serializer (a:Type) = ps_a:parser_serializer_unit a{is_not_unit ps_a}
+let is_not_unit (#bytes:Type0) {|bytes_like bytes|} (#a:Type) (ps_a:parser_serializer_unit bytes a) = ps_a.parse empty == None
+let parser_serializer (bytes:Type0) {|bytes_like bytes|} (a:Type) = ps_a:parser_serializer_unit bytes a{is_not_unit ps_a}
 
 (*** Parser combinators ***)
 
-val bind: #a:Type -> #b:(a -> Type) -> ps_a:parser_serializer_unit a -> ps_b:(xa:a -> parser_serializer_unit (b xa)) -> Pure (parser_serializer_unit (xa:a&(b xa)))
+val bind: #a:Type -> #b:(a -> Type) -> #bytes:Type0 -> {| bytes_like bytes |} -> ps_a:parser_serializer_unit bytes a -> ps_b:(xa:a -> parser_serializer_unit bytes (b xa)) -> Pure (parser_serializer_unit bytes (xa:a&(b xa)))
   (requires True)
   (ensures fun res -> is_not_unit res <==> is_not_unit ps_a \/ (forall xa. is_not_unit (ps_b xa)))
+
 val isomorphism_explicit:
-  #a:Type -> b:Type -> ps_a:parser_serializer_unit a -> f:(a -> b) -> g:(b -> a) ->
+  #a:Type -> #bytes:Type0 -> {| bytes_like bytes |} -> b:Type ->
+  ps_a:parser_serializer_unit bytes a -> f:(a -> b) -> g:(b -> a) ->
   g_f_inv:(xa:a -> Lemma (g (f xa) == xa)) -> f_g_inv:(xb:b -> Lemma (f (g xb) == xb)) ->
-  Pure (parser_serializer_unit b) (requires True) (ensures fun res -> is_not_unit res <==> is_not_unit ps_a)
-val isomorphism: #a:Type -> b:Type -> ps_a:parser_serializer_unit a -> f:(a -> b) -> g:(b -> a) -> Pure (parser_serializer_unit b)
+  Pure (parser_serializer_unit bytes b) (requires True) (ensures fun res -> is_not_unit res <==> is_not_unit ps_a)
+
+val isomorphism:
+  #a:Type -> #bytes:Type0 -> {| bytes_like bytes |} -> b:Type ->
+  ps_a:parser_serializer_unit bytes a -> f:(a -> b) -> g:(b -> a) ->
+  Pure (parser_serializer_unit bytes b)
   (requires (forall xa. g (f xa) == xa) /\ (forall xb. f (g xb) == xb))
   (ensures fun res -> is_not_unit res <==> is_not_unit ps_a)
 
 (*** Parser for basic types ***)
 
-val ps_unit: parser_serializer_unit unit
+val ps_unit: #bytes:Type0 -> {| bytes_like bytes |} -> parser_serializer_unit bytes unit
 
-val ps_lbytes: n:nat{1 <= n} -> parser_serializer (lbytes n)
+type lbytes (bytes:Type0) {|bytes_like bytes|} (n:nat) = b:bytes{length b == n}
+val ps_lbytes: #bytes:Type0 -> {| bytes_like bytes |} -> n:nat{1 <= n} -> parser_serializer bytes (lbytes bytes n)
 
 //val ps_u8: parser_serializer uint8
 //val ps_u16: parser_serializer uint16
@@ -98,11 +82,11 @@ val ps_lbytes: n:nat{1 <= n} -> parser_serializer (lbytes n)
 
 (*** Exact parsers ***)
 
-type bare_parser_exact (a:Type) = b:bytes -> option a
-type bare_serializer_exact (a:Type) = a -> bytes
-noeq type parser_serializer_exact (a:Type) = {
-  parse_exact: bare_parser_exact a;
-  serialize_exact: bare_serializer_exact a;
+type bare_parser_exact (bytes:Type0) {|bytes_like bytes|} (a:Type) = b:bytes -> option a
+type bare_serializer_exact (bytes:Type0) {|bytes_like bytes|} (a:Type) = a -> bytes
+noeq type parser_serializer_exact (bytes:Type0) {|bytes_like bytes|} (a:Type) = {
+  parse_exact: bare_parser_exact bytes a;
+  serialize_exact: bare_serializer_exact bytes a;
   parse_serialize_inv_exact: x:a -> Lemma (
     parse_exact (serialize_exact x) == Some x
   );
@@ -113,8 +97,8 @@ noeq type parser_serializer_exact (a:Type) = {
   );
 }
 
-val ps_to_pse: #a:Type -> parser_serializer_unit a -> parser_serializer_exact a
-val pse_list: #a:Type -> ps_a:parser_serializer a -> parser_serializer_exact (list a)
+val ps_to_pse: #bytes:Type0 -> {|bytes_like bytes|} -> #a:Type -> parser_serializer_unit bytes a -> parser_serializer_exact bytes a
+val pse_list: #bytes:Type0 -> {|bytes_like bytes|} -> #a:Type -> ps_a:parser_serializer bytes a -> parser_serializer_exact bytes (list a)
 
 (*** Parser for variable-length lists ***)
 
@@ -126,12 +110,12 @@ type size_range = {
 let in_range (r:size_range) (x:nat) =
   r.min <= x && x <= r.max
 
-let rec byte_length (#a:Type) (ps_a:parser_serializer a) (l:list a) : nat =
+let rec byte_length (#bytes:Type0) {|bytes_like bytes|} (#a:Type) (ps_a:parser_serializer bytes a) (l:list a) : nat =
   match l with
   | [] -> 0
-  | h::t -> bytes_length (ps_a.serialize h bytes_empty) + byte_length ps_a t
+  | h::t -> length (add_prefixes (ps_a.serialize h) empty <: bytes) + byte_length ps_a t
 
-type blseq (a:Type) (ps_a:parser_serializer a) (r:size_range) = s:Seq.seq a{in_range r (byte_length ps_a (Seq.seq_to_list s))}
-type blbytes (r:size_range) = b:bytes{in_range r (bytes_length b)}
-val ps_seq: #a:Type -> r:size_range -> ps_a:parser_serializer a -> parser_serializer (blseq a ps_a r)
-val ps_bytes: r:size_range -> parser_serializer (blbytes r)
+type blseq (#bytes:Type0) {|bytes_like bytes|} (a:Type) (ps_a:parser_serializer bytes a) (r:size_range) = s:Seq.seq a{in_range r (byte_length ps_a (Seq.seq_to_list s))}
+type blbytes (bytes:Type0) {|bytes_like bytes|} (r:size_range) = b:bytes{in_range r (length b)}
+val ps_seq: #bytes:Type0 -> {|bytes_like bytes|} -> #a:Type -> r:size_range -> ps_a:parser_serializer bytes a -> parser_serializer bytes (blseq a ps_a r)
+val ps_bytes: #bytes:Type0 -> {|bytes_like bytes|} -> r:size_range -> parser_serializer bytes (blbytes bytes r)
