MLS.Bytes.fsti
@@ -12,6 +12,8 @@ class bytes_like (bytes:Type0) = {
   concat: bytes -> bytes -> bytes;
   concat_length: b1:bytes -> b2:bytes -> Lemma (length (concat b1 b2) == (length b1) + (length b2));
 
+  concat_empty_left: b:bytes -> Lemma (concat empty b == b);
+
   slice: b:bytes -> i:nat -> j:nat{i <= j /\ j <= length b} -> bytes;
   slice_length: b:bytes -> i:nat -> j:nat{i <= j /\ j <= length b} -> Lemma (length (slice b i j) == j-i);
 
@@ -24,5 +26,32 @@ class bytes_like (bytes:Type0) = {
 
   concat_slice: b:bytes -> i:nat{i <= length b} -> Lemma
     (concat (slice b 0 i) (slice b i (length b)) == b);
+
+  //is_public: bytes -> Type0;
+  //to_nat: b:bytes{is_public b} -> nat;
+  //from_nat: nat -> b:bytes{is_public b};
 }
 
+open FStar.Seq
+
+instance seq_bytes_like (a:Type0): bytes_like (Seq.seq a) =
+  {
+    length = Seq.length;
+
+    empty = Seq.empty;
+    empty_length = (fun () -> ());
+    length_zero = (fun b -> assert(Seq.equal b Seq.empty));
+
+    concat = Seq.append;
+    concat_length = (fun b1 b2 -> ());
+
+    concat_empty_left = (fun b -> assert(Seq.equal (Seq.append Seq.empty b) b));
+
+    slice = Seq.slice;
+    slice_length = (fun b i j -> ());
+
+    slice_concat_left = (fun b1 b2 -> assert(Seq.equal (Seq.slice (Seq.append b1 b2) 0 (Seq.length b1)) b1));
+    slice_concat_right = (fun b1 b2 -> assert(Seq.equal (Seq.slice (Seq.append b1 b2) (Seq.length b1) (Seq.length (Seq.append b1 b2))) b2));
+
+    concat_slice = (fun b i -> assert(Seq.equal (Seq.append (Seq.slice b 0 i) (Seq.slice b i (Seq.length b))) b));
+  }
